In each of Problems 1 through 6, determine the order of the given differential
equation; also state whether the equation is linear or nonlinear.
\begin{enumerate}
%%%%%%%%%%%%%%%%%%%%%%%%%%%%%%%%%%%%%1.3.1%%%%%%%%%%%%%%%%%%%%%%%%%%%%%%%%%%%%%%
   \item[1.3.1]   $t^2\frac{d^2y}{dt^2} + t\frac{dy}{dt} + 2y = \sin(t)$. \\

      \textbf{Answer.} Linear of order 2.
%%%%%%%%%%%%%%%%%%%%%%%%%%%%%%%%%%%%%1.3.2%%%%%%%%%%%%%%%%%%%%%%%%%%%%%%%%%%%%%%
   \item[1.3.2]   $(1 + y^2)\frac{d^2y}{dt^2} + t\frac{dy}{dt} + y =e^t$. \\

      \textbf{Answer.} Nonlinear of order 2.
%%%%%%%%%%%%%%%%%%%%%%%%%%%%%%%%%%%%%1.3.3%%%%%%%%%%%%%%%%%%%%%%%%%%%%%%%%%%%%%%
   \item[1.3.3]   $\frac{d^4y}{dt^4} + \frac{d^3y}{dt^3} + \frac{d^2y}{dt^2} +
                   \frac{dy}{dt} + y = 1$. \\

      \textbf{Answer.} Linear of order 4.
%%%%%%%%%%%%%%%%%%%%%%%%%%%%%%%%%%%%%1.3.4%%%%%%%%%%%%%%%%%%%%%%%%%%%%%%%%%%%%%%
   \item[1.3.4]   $\frac{dy}{dt} + ty^2 = 0$. \\

      \textbf{Answer.} Nonlinear of order 1.
%%%%%%%%%%%%%%%%%%%%%%%%%%%%%%%%%%%%%1.3.5%%%%%%%%%%%%%%%%%%%%%%%%%%%%%%%%%%%%%%
   \item[1.3.5]   $\frac{d^2y}{dt^2} + \sin(t + y) = \sin(t)$. \\

      \textbf{Answer.} Nonlinear of order 2.
%%%%%%%%%%%%%%%%%%%%%%%%%%%%%%%%%%%%%1.3.6%%%%%%%%%%%%%%%%%%%%%%%%%%%%%%%%%%%%%%
   \item[1.3.6]   $\frac{d^3y}{dt^3} + t\frac{dy}{dt} + (\cos^2(t))y = t^3$. \\

      \textbf{Answer.} Linear of order 3.
\end{enumerate}

In problems 8 and 11, verify that each given function is a solution of the
differential equation.
\begin{enumerate}
%%%%%%%%%%%%%%%%%%%%%%%%%%%%%%%%%%%%%1.3.8%%%%%%%%%%%%%%%%%%%%%%%%%%%%%%%%%%%%%%
   \item[1.3.8]   $y'' + 2y' - 3y = 0; \quad y_1(t) = e^{-3t},
                                       \quad y_2(t) = e^t$. \\

      \textbf{Solution.} We have
      $${y_1}' = -3e^{-3t} \text{ and } {y_1}'' = 9e^{-3t},$$
      so that
      $${y_1}'' + 2{y_1}' - 3y_1 = 9e^{-3t} + 2(-3e^{-3t}) - 3e^{-3t} = 0.$$
      Similarly,
      $${y_2}' = {y_2}'' = e^t,$$
      so that
      $${y_2}'' + 2{y_2}' - 3y_2 = e^t + 2e^t - 3e^t = 0.$$
      That is, $y_1$ and $y_2$ both satisfy the given differential equations.
      
%%%%%%%%%%%%%%%%%%%%%%%%%%%%%%%%%%%%%1.3.11%%%%%%%%%%%%%%%%%%%%%%%%%%%%%%%%%%%%%
   \item[1.3.11]  $2t^2y'' + 3ty' - y = 0, \quad t > 0; \quad y_1(t) = t^{1/2}, 
                                           \quad y_2(t) = t^{-1}$. \\

      \textbf{Solution.} For $t > 0$, we have
      $${y_1}' = \frac{1}{2\sqrt{t}} \text{ and }
        {y_1}'' = -\frac{1}{4\sqrt{t^3}},$$
      so that
      \begin{align*}
         2t^2{y_1}'' + 3t{y_1}' - {y_1} &= -2t^2\frac{1}{4\sqrt{t^3}} +
            3t\frac{1}{2\sqrt{t}} - \sqrt{t} \\
            &= -\frac{2}{4}t^{1/2} + \frac{3}{2}t^{1/2} - t^{1/2} \\
            &= \left(-\frac{2}{4} + \frac{3}{2} - 1\right)t^{1/2} \\
            & = 0 \cdot t^{1/2} = 0,
      \end{align*}

      and
      $${y_2}' = -t^{-2} \text{ and } {y_2}'' = 2t^{-3},$$
      so that
      \begin{align*}
         2t^2{y_2}'' + 3t{y_2}' - {y_2} &= 2t^2(2t^{-3}) +
            3t(-t^{-2}) - t^{-1} \\
            &= 4t^{-1} - 3t^{-1} - t^{-1} \\
            &= (4 - 3 - 1)t^{-1} = 0 \cdot t^{-1} = 0.
      \end{align*}
\end{enumerate}
