\documentclass[9pt]{article}

\usepackage{amssymb}
\usepackage{amsmath}
\usepackage{amsfonts}
\usepackage{comment}
\usepackage{fancyhdr}
\usepackage{mathrsfs}
\usepackage{amscd}
%\usepackage[retainorgcmds]{IEEEtrantools}

\everymath{\displaystyle}

\usepackage{tikz}

\voffset = -50pt
%\textheight = 700pt
\addtolength{\textwidth}{60pt}
\addtolength{\evensidemargin}{-30pt}
\addtolength{\oddsidemargin}{-30pt}
%\setlength{\headheight}{44pt}

\pagestyle{fancy}
\fancyhf{} % clear all fields
\fancyhead[R]{%
  \scshape
  \begin{tabular}[t]{@{}r@{}}
  MATH 545, Spring 2016\\Section 1 (9515)\\
  HW \#6, DUE: 2016, February 22
  \end{tabular}}
\fancyhead[L]{%
  \scshape
  \begin{tabular}[t]{@{}r@{}}
  JOSEPH OKONOBOH\\Mathematics\\Cal State Long Beach
  \end{tabular}}
\fancyfoot[C]{\thepage}

\newcommand{\qed}{\hfill \ensuremath{\Box}}


\newcommand*\circled[1]{\tikz[baseline=(char.base)]{
            \node[shape=circle,draw,inner sep=2pt] (char) {#1};}}


\newcommand{\cyc}[1]{\langle #1 \rangle}
\newcommand{\Z}{\mathbb{Z}}
\newcommand{\I}{\mathbb{I}}
\newcommand{\F}{\mathbb{F}}
\newcommand{\M}{\mathbb{M}}
\newcommand{\R}{\mathbb{R}}
\newcommand{\Q}{\mathbb{Q}}
\newcommand{\Ker}{\text{Ker}}
\newcommand{\Coker}{\text{Coker}}
\newcommand{\im}{\text{Im}}
\newcommand{\D}{\displaystyle}
\DeclareTextCommand{\_}{OT1}{%
  \leavevmode \kern.06em\vbox{\hrule width.6em}}
%\setcounter{section}{-1}

\begin{document}
\begin{enumerate}
%%%%%%%%%%%%%%%%%%%%%%%%%%%%%%%%%%%%%%%15%%%%%%%%%%%%%%%%%%%%%%%%%%%%%%%%%%%%%%%
   \item[15.]  Show that the Snake Lemma sequence is exact at $\Coker(\gamma')$.

      \textbf{Proof.} It suffices to show that
      $\im(\partial) = \Ker(\varphi')$. So we will show each set is
      contained in the other.
      \begin{itemize}
         \item ($\subseteq$): Let $x \in \im(\partial)$. Then
               $x = \partial(k'')$, for some $k'' \in \Ker(\gamma'')$. From our
               definition of $\partial$, it follows that there exist $m \in M$
               and $n' \in N'$ such that $\beta(m) = k''$,
               $\gamma(m) = \alpha(n')$ and $\partial(k'') =n' + \im(\gamma')$.
               So
               \begin{align*}
                  \varphi'(\partial(k'')) &= \varphi'(n'+\im(\gamma')) \\
                     &= \alpha'(n') + \im(\gamma) \\
                     &= \gamma(m) + \im(\gamma) \\
                     &= \im(\gamma) &[\gamma(m) \in \im(\gamma)] \\
                     &= 0,
               \end{align*}
               so that $x \in \Ker(\varphi')$. Thus 
               $\im(\partial) \subseteq \Ker(\varphi')$.
         \item ($\supseteq$): Let $y \in \Ker(\varphi')$, where
               $y = s' + \im(\gamma')$ for some $s' \in N'$. Since
               $y \in \Ker(\varphi')$, it follows that
               $$\im(\gamma) = 0 = \varphi'(y) = \varphi'(s' + \im(\gamma')) =
                 \alpha'(s') + \im(\gamma),$$
               so that $\alpha'(s') \in \im(\gamma)$. That is,
               $\alpha'(s') = \gamma(t)$ for some $t \in M$. Now we have that
               \begin{align*}
                  0 &= \beta'(\alpha'(s')) &[\im(\alpha')=\Ker(\beta')] \\
                    &= \beta'(\gamma(t)) \\
                    &= \gamma''(\beta(t)), &[\text{Commutativity}]                    
               \end{align*}
               so that $d'' \in \Ker(\gamma'')$, where $d'' = \beta(t)$. By the
               definition of $\partial$, it follows that
               $y = s' + \im(\gamma') = \partial(d'') \in \im(\partial)$. Thus,
               $\im(\partial) \supseteq \Ker(\varphi')$.
      \end{itemize}
      Conclude that $\im(\partial) = \Ker(\varphi')$. That is, the
      Snake Lemma sequence is exact at $\Coker(\gamma')$. \qed
%%%%%%%%%%%%%%%%%%%%%%%%%%%%%%%%%%%%%%%16%%%%%%%%%%%%%%%%%%%%%%%%%%%%%%%%%%%%%%%
   \item[16.]  Let
               $$0 \rightarrow M' \stackrel{\alpha}{\longrightarrow} M
               \stackrel{\beta}{\longrightarrow} M'' \rightarrow 0$$
               be a short exact sequence, and $N$ a module. Show that the
               sequence
               $$0 \rightarrow \text{Hom}(M'', N) \stackrel{\_\circ\beta}
               {\longrightarrow} \text{Hom}(M, N)
               \stackrel{\_\circ\alpha}{\longrightarrow} \text{Hom}(M', N).$$
               is exact.
               
      \textbf{Proof.} It suffices to show that $\_\circ\beta$ is injective and
      that $\im(\_\circ\beta) = \Ker(\_\circ\alpha)$. Since $\beta$ is onto, the
      former follows by our discussion in class, so it remains to show the
      latter.
      
      \begin{itemize}
         \item \textbf{Show that } $\im(\_\circ\beta) = \Ker(\_\circ\alpha)$.
               \begin{itemize}
                  \item $(\subseteq):$ Let $\gamma \in \im(\_\circ\beta)$. Then
                        $\gamma = \phi\circ\beta$ for some
                        $\phi \in \text{Hom}(M'', N)$. It follows that
                        \begin{align*}
                           (\_\circ\alpha)(\gamma) &= \gamma \circ \alpha \\
                              &= (\phi\circ\beta)\circ\alpha \\
                              &= \phi\circ(\beta\circ\alpha) \\
                              &= 0,
                        \end{align*}
                        where the last equality follows because
                        $\beta\circ\alpha$ is a zero map
                        (since $\im(\alpha) = \Ker(\beta)$) and because every
                        module maps 0 to 0. That is,
                        $\gamma \in \Ker(\_\circ\alpha)$, and thus,
                        $\im(\_\circ\beta) \subseteq \Ker(\_\circ\alpha)$.
                  \item $(\supseteq):$ Let $\sigma \in \Ker(\_\circ\alpha)$, so
                        that $(\_\circ\alpha)(\sigma) = \sigma\circ\alpha = 0$.
                        Define a function $\delta : M'' \rightarrow N$, such
                        that if $m'' \in M''$, then $\delta(m'') = \sigma(m)$,
                        where $m'' = \beta(m)$, for some $m \in M$. Observe that
                        $(\delta\circ\beta)(m) = \sigma(m)$ for all $m \in M$,
                        so that $\delta\circ\beta = \sigma$. Also observe that
                        since $\beta$ is onto, the function $\delta$ is defined for every
                        $m'' \in M$. It remains to show
                        that $\delta \in \text{Hom}(M'', N)$; that is, we must
                        show that $\delta$ is a well defined $R$-module
                        homomorphism.
                        \begin{itemize}
                           \item \textbf{$\delta$ is well-defined.} Let $m'' \in M$;
                                 Since $\beta$ is onto, there exists $m_1 \in M$
                                 such that $m'' = \beta(m_1)$. Now suppose that
                                 $\beta(m_1) = \beta(m_2)$ for some
                                 $m_2 \in M$. It suffices to show that
                                 $\sigma(m_1) = \sigma(m_2)$. Since
                                 $\beta(m_1) = \beta(m_2)$, it follows that
                                 $m_1 - m_2 \in \Ker(\beta) = \im(\alpha)$, so
                                 that $m_1 - m_2 = \alpha(t')$ for some
                                 $t' \in M'$. Since $\sigma\circ\alpha = 0$, it
                                 follows that
                                 $$\sigma(m_1) - \sigma(m_2) = \sigma(m_1 - m_2)
                                 = \sigma(\alpha(t')) = 0,$$
                                 so that $\sigma(m_1) = \sigma(m_2)$, and thus,
                                 $\delta$ is well-defined.
                           
                           \item \textbf{$\delta$ is an $R$-module
                                 homomorphism.} Let $r \in R$ and let
                                 $a'', b'' \in M''$. Thus $\delta(a'') = \sigma(a)$ and
                                 $\delta(b'') = \sigma(b)$, where $\beta(a) = a''$
                                 and $\beta(b) = b''$, for some $a, b \in M$.
                                 Thus
                                 \begin{align*}
                                    \delta(a''+b'')&=\delta(\beta(a)+\beta(b))\\
                                       &= \delta(\beta(a+b)) \\
                                       &= \sigma(a+b) \\
                                       &= \sigma(a)+\sigma(b)\\
                                       &= \delta(a'')+\delta(b''),
                                 \end{align*}
                                 and
                                 $$\delta(ra'') = \delta(r\beta(a)) =
                                   \delta(\beta(ra)) = \sigma(ra) = r\sigma(a)
                                   = r\delta(a'').$$
                                 That is, $\delta$ is an $R$-module homomorphism.
                                 Hence $\delta \in \text{Hom}(M'', N)$.
                        \end{itemize}
                        Since  $\delta\circ\beta = \sigma$, it follows that
                        $\sigma \in \im (\_\circ\beta)$, so that
                        $\im(\_\circ\beta) \supseteq \Ker(\_\circ\alpha)$.
               \end{itemize}
               Conclude that $\im(\_\circ\beta) = \Ker(\_\circ\alpha)$.
      \end{itemize}
      Thus the sequence 
               $$0 \rightarrow \text{Hom}(M'', N) \stackrel{\_\circ\beta}
               {\longrightarrow} \text{Hom}(M, N)
               \stackrel{\_\circ\alpha}{\longrightarrow} \text{Hom}(M', N)$$
               is exact. \qed
\end{enumerate}
\end{document}
